proof/InternalLemmas2.v
@@ -1,0 +1,1790 @@
+(*******************************************************************************)
+(*  © Université Lille 1, The Pip Development Team (2015-2018)                 *)
+(*                                                                             *)
+(*  This software is a computer program whose purpose is to run a minimal,     *)
+(*  hypervisor relying on proven properties such as memory isolation.          *)
+(*                                                                             *)
+(*  This software is governed by the CeCILL license under French law and       *)
+(*  abiding by the rules of distribution of free software.  You can  use,      *)
+(*  modify and/ or redistribute the software under the terms of the CeCILL     *)
+(*  license as circulated by CEA, CNRS and INRIA at the following URL          *)
+(*  "http://www.cecill.info".                                                  *)
+(*                                                                             *)
+(*  As a counterpart to the access to the source code and  rights to copy,     *)
+(*  modify and redistribute granted by the license, users are provided only    *)
+(*  with a limited warranty  and the software's author,  the holder of the     *)
+(*  economic rights,  and the successive licensors  have only  limited         *)
+(*  liability.                                                                 *)
+(*                                                                             *)
+(*  In this respect, the user's attention is drawn to the risks associated     *)
+(*  with loading,  using,  modifying and/or developing or reproducing the      *)
+(*  software by the user in light of its specific status of free software,     *)
+(*  that may mean  that it is complicated to manipulate,  and  that  also      *)
+(*  therefore means  that it is reserved for developers  and  experienced      *)
+(*  professionals having in-depth computer knowledge. Users are therefore      *)
+(*  encouraged to load and test the software's suitability as regards their    *)
+(*  requirements in conditions enabling the security of their systems and/or   *)
+(*  data to be ensured and,  more generally, to use and operate it in the      *)
+(*  same conditions as regards security.                                       *)
+(*                                                                             *)
+(*  The fact that you are presently reading this means that you have had       *)
+(*  knowledge of the CeCILL license and that you accept its terms.             *)
+(*******************************************************************************)
+
+(** * Summary 
+    This file contains several internal lemmas to help prove invariants *)
+Require Import Model.ADT Isolation Consistency WeakestPreconditions List 
+Core.Internal  Model.MAL StateLib Model.Hardware 
+ DependentTypeLemmas Model.Lib Invariants Lib PropagatedProperties InternalLemmas.
+Require Import Coq.Logic.ProofIrrelevance Omega Classical_Prop.
+
+Import List.ListNotations.
+ Lemma getIndirectionStop1' s indirection x idxind va l entry :
+StateLib.Level.eqb l fstLevel = false ->  indirection <> defaultPage ->
+lookup indirection idxind (memory s) beqPage beqIndex = Some (PE x) ->
+isEntryPage indirection idxind entry s ->
+StateLib.getIndexOfAddr va l  =  idxind ->
+StateLib.getIndirection indirection va l 1 s = Some  entry.
+Proof.
+intros Hlnotzero Hindnotnull Hlookup Hep Hidx .
+unfold isEntryPage in *.
+rewrite Hlookup in Hep. subst entry.
+unfold StateLib.getIndirection.
+  case_eq (StateLib.Level.eqb l fstLevel).
+  - intros H2. rewrite H2 in Hlnotzero.
+    contradict Hlnotzero.  intuition.
+  - intros H2.
+    unfold  StateLib.getIndexOfAddr in *.
+    case_eq ( ge_dec l (length va)).
+    * intros.
+      destruct va.
+      simpl in *.
+      subst.
+      destruct l. simpl in *.
+      contradict H.
+      omega.
+   * unfold runvalue in Hidx.
+     intros.
+     unfold StateLib.readPhyEntry.
+     inversion Hidx.
+     rewrite H0.
+     rewrite Hlookup.
+     case_eq(defaultPage =? pa x).
+     intros.
+     apply beq_nat_true in H1.
+     f_equal.
+     unfold defaultPage in *.
+     unfold CPage.
+     unfold CPage in H1.
+     destruct(lt_dec 0 nbPage).
+     subst.
+     simpl in *.
+     destruct x.
+     simpl in *.
+     subst.
+     destruct pa.
+     simpl in *.
+     subst.
+     assert (Hp = ADT.CPage_obligation_1 0 l0).
+     apply proof_irrelevance.
+     subst.
+     reflexivity.
+     destruct page_d.
+     destruct pa.
+     simpl in *.
+     subst.
+     assert (Hp0 = Hp).
+     apply proof_irrelevance.
+     subst. reflexivity.
+     intros.
+     unfold StateLib.Level.pred.
+     case_eq (gt_dec l 0).
+     intros g H4; reflexivity.
+     intros.
+     subst.
+     apply levelEqBEqNatFalse0 in H2.
+     contradict H2.
+     assumption.  
+
+Qed.
+
+ Lemma getIndirectionStopS' :
+forall  stop (s : state) (nbL : level)  nextind pd va indirection,
+stop + 1 <= nbL -> indirection <> defaultPage ->
+StateLib.getIndirection pd va nbL stop s = Some indirection->
+StateLib.getIndirection indirection va (CLevel (nbL - stop)) 1 s = Some nextind ->  
+StateLib.getIndirection pd va nbL (stop + 1) s = Some nextind.
+Proof.
+induction stop.
+- intros. simpl.
+  cbn in *.
+  inversion H1.
+  subst.
+  rewrite NPeano.Nat.sub_0_r in H2.
+  unfold CLevel in H2.
+  destruct (lt_dec nbL nbLevel ).
+  simpl in *.
+  destruct nbL.
+  simpl in *.
+  assert (Hl = ADT.CLevel_obligation_1 l0 l ).
+  apply proof_irrelevance.
+  subst.
+  assumption.
+  destruct nbL. simpl in *.
+  contradict n.
+  omega.
+- intros.
+  simpl .
+  simpl in H1.
+  case_eq (StateLib.Level.eqb nbL fstLevel).
+  + intros. rewrite <- H2.
+    inversion H1.
+    subst.
+    symmetry.
+    rewrite H3 in H5. inversion H5. subst.
+    simpl. clear H1.
+    apply levelEqBEqNatTrue in H3.
+    case_eq (StateLib.Level.eqb (CLevel (nbL - S stop)) fstLevel).
+    intros.
+    reflexivity.
+    intros.
+    apply levelEqBEqNatFalse0 in H1.
+   
+    contradict H1.
+    unfold CLevel.
+    case_eq ( lt_dec (nbL - S stop) nbLevel ).
+    intros. simpl . rewrite H3.
+    unfold fstLevel.
+    unfold CLevel.
+    case_eq(lt_dec 0 nbLevel ).
+    intros.
+    simpl. omega.
+    intros.
+    assert(0 < nbLevel).
+    apply nbLevelNotZero.
+    contradict H6. omega.
+    intros.  
+    Opaque StateLib.getIndirection.
+    simpl in *.
+    unfold fstLevel in H3.
+    unfold CLevel in H3.
+    case_eq (lt_dec 0 nbLevel).
+    intros.
+    rewrite H4 in H3.
+    simpl in *.
+    destruct nbL.
+    simpl in *.
+    subst.
+    inversion H3.
+    subst. omega.
+    intros.
+    assert (0 < nbLevel).
+    apply nbLevelNotZero.
+    omega.
+  + intros Hftlevel.  
+    rewrite Hftlevel in H1.
+    case_eq (StateLib.readPhyEntry pd (StateLib.getIndexOfAddr va nbL) (memory s)).
+    { intros. rewrite H3 in H1.
+      case_eq ( defaultPage =? p).
+      - intros. rewrite H4 in H1.
+        inversion H1.
+       contradict H0. intuition.
+      - intros. rewrite H4 in H1.
+        case_eq (StateLib.Level.pred nbL ).
+        + intros. rewrite H5 in H1.
+          unfold StateLib.Level.pred in H5.
+          case_eq (gt_dec nbL 0).
+          intros.
+          rewrite H6 in H5.
+          generalize (IHstop s l nextind p va indirection);clear IHstop;intros IHstop.
+          apply IHstop.
+          inversion H5.
+          simpl in *.
+          omega.
+          assumption.
+          assumption.
+          clear IHstop.
+          inversion H5.
+          Opaque StateLib.getIndirection.
+          simpl in *.
+          subst.
+          replace (nbL - 1 - stop) with (nbL - S stop).
+          assumption.
+          omega.
+          intros.
+          apply levelEqBEqNatFalse0 in Hftlevel.
+          contradict Hftlevel.
+          omega.
+          Transparent StateLib.getIndirection.
+        + intros.  rewrite H5 in H1. inversion H1.  
+   
+     }
+     { intros. rewrite H3 in H1.    inversion H1. }
+Qed.
+Lemma indirectionDescriptionInGetIndirections indirection pd partition vaToPrepare l s root:
+(root=PDidx\/ root=sh1idx \/ root=sh2idx) ->
+nextEntryIsPP partition root pd s ->
+indirectionDescription s partition indirection root vaToPrepare l ->
+In indirection (getIndirections pd s).
+Proof.
+intros Horroot Hpd Hind.
+unfold indirectionDescription in *.
+destruct Hind as (tableroot & Hpp & Hrootnotdef & Hor).
+ assert(Hpdor: tableroot=pd).
+ { destruct Horroot as [Horroot | [Horroot | Horroot]];subst.
+  apply getPdNextEntryIsPPEq with partition s;trivial.
+  apply nextEntryIsPPgetPd;trivial.
+  apply getSh1NextEntryIsPPEq with partition s;trivial. 
+  apply nextEntryIsPPgetFstShadow;trivial. 
+  apply getSh2NextEntryIsPPEq with partition s;trivial. 
+  apply nextEntryIsPPgetSndShadow;trivial. 
+  }
+  subst tableroot.
+  destruct Hor as [Hor | Hor].
+  + clear Horroot.
+  intuition;subst.
+  unfold getIndirections.
+  pose proof nbLevelNotZero.
+  destruct  nbLevel;simpl. omega.
+  left;trivial.
+  +
+destruct Hor as (nbL & stop & Hnbl & Hstop & Hind & Hdef & Hl).
+apply getIndirectionInGetIndirections with vaToPrepare nbL stop;trivial.
+apply nbLevelNotZero.
+  apply getNbLevelLe;trivial.
+Qed.
+
+Lemma getIndirectionProp' :
+forall stop s nextind idxind indirection pd va (nbL : level) entry,
+stop +1 <= nbL -> indirection <> defaultPage ->
+StateLib.Level.eqb (CLevel (nbL - stop)) fstLevel = false ->
+StateLib.getIndexOfAddr va (CLevel (nbL - stop)) = idxind ->
+lookup indirection idxind (memory s) beqPage beqIndex = Some (PE entry)->
+isEntryPage  indirection idxind nextind s ->
+StateLib.getIndirection pd va nbL stop s = Some indirection ->
+StateLib.getIndirection pd va nbL (stop + 1) s = Some nextind.
+Proof.
+intros.
+apply getIndirectionStopS' with indirection;trivial.
+apply getIndirectionStop1'  with entry idxind ;trivial.
+Qed.
+
+
+Lemma beq_nat_falseNot (tbl:page) :
+(defaultPage =? tbl) = false -> tbl <> defaultPage.
+Proof.
+intros.
+apply beq_nat_false in H.
+unfold not;intros;subst.
+now contradict H.
+Qed.
+Lemma getIndirectionEqStop :
+forall (stop : nat) (nbL : level) (va1 va2 : vaddr) (pd : page)  (s : state),
+stop <= nbL ->
+StateLib.checkVAddrsEqualityWOOffset stop va1 va2 nbL = true ->
+getIndirection pd va1 nbL stop s = getIndirection pd va2 nbL stop s.
+Proof.
+(* intro.
+assert(Hgen: stop <= stop) by omega.
+revert Hgen.
+generalize stop at 1 4. *)
+induction stop;simpl;intros;trivial.
+case_eq(StateLib.Level.eqb nbL fstLevel);intros * Hl;trivial;rewrite Hl in *.
+case_eq(StateLib.Level.pred nbL);intros * Hlpred;rewrite Hlpred in *.
++ case_eq (StateLib.getIndexOfAddr va1 nbL =? StateLib.getIndexOfAddr va2 nbL);intros * Hvas;rewrite Hvas in *;
+try now contradict H0.
+apply beq_nat_true in Hvas.
+destruct(StateLib.getIndexOfAddr va1 nbL);simpl in *.
+destruct(StateLib.getIndexOfAddr va2 nbL);simpl in *.
+subst.
+assert(Hi = Hi0) by apply proof_irrelevance.
+subst.
+destruct (StateLib.readPhyEntry pd {| i := i0; Hi := Hi0 |} (memory s));trivial.
+destruct( defaultPage =? p );trivial.
+apply IHstop;trivial.
+apply levelPredMinus1 in Hlpred;trivial.
+symmetry in Hlpred.
+unfold CLevel in *.
+case_eq(lt_dec (nbL - 1) nbLevel );intros * Hcl;rewrite Hcl in *.
+simpl in *.
+destruct l;simpl in *.
+inversion Hlpred.
+subst.
+omega.
+destruct nbL;simpl in *.
+omega.
++ apply levelPredNone in Hl;trivial.
+contradict Hl.
+trivial.
+Qed.
+
+Lemma noDupPreviousMMULevels s:
+forall m n pd,
+NoDup(getIndirectionsAux pd s m) ->
+n  <= m ->
+NoDup(getIndirectionsAux pd s n ).
+Proof.
+induction m;simpl;intros.
++
+replace n with 0 by omega.
+simpl.
+constructor.
++
+revert dependent pd.
+revert H0.
+induction n.
+-
+intros.
+simpl.
+constructor.
+-
+intros.
+simpl.
+apply NoDup_cons_iff in H.
+destruct H.
+rewrite in_flat_map in H.
+constructor.
+*
+rewrite in_flat_map.
+contradict H.
+destruct H as (x & Hxtrue & Hxfalse).
+exists x.
+split;trivial.
+
+
+pose proof inclGetIndirectionsAuxLe.
+unfold incl in *.
+apply H with n;trivial.
+omega.
+* clear H.
+induction (getTablePages pd tableSize s);simpl.
+constructor.
+simpl in *.
+apply NoDupSplitInclIff in H1.
+intuition.
+apply NoDupSplitInclIff.
+intuition.
+unfold disjoint in *.
+intros.
+rewrite in_flat_map.
+contradict H4.
+unfold not;intros.
+destruct H4 as (x0 & Hx0 & Hx00).
+pose proof inclGetIndirectionsAuxLe.
+unfold incl in *.
+
+assert(Htrue: ~ In x (flat_map (fun p : page => getIndirectionsAux p s m) l)).
+apply H2.
+apply H4 with n;trivial.
+omega.
+contradict Htrue.
+rewrite in_flat_map.
+exists x0;split;trivial.
+apply H4 with n;trivial.
+omega.
+Qed.
+
+Lemma indirectionNotInPreviousMMULevel' s (ptVaChildpd:page) idxvaChild (* phyVaChild *)  
+  pdChildphy (* currentPart *)
+(* presentvaChild *) vaChild phyDescChild level (* entry *):
+ partitionDescriptorEntry s ->
+ isPresentNotDefaultIff s ->
+ noDupConfigPagesList s ->
+configTablesAreDifferent s ->
+(* In currentPart (getPartitions multiplexer s) ->  *)
+(* In phyVaChild (getAccessibleMappedPages currentPart s) -> *)
+(* lookup ptVaChildpd idxvaChild (memory s) beqPage beqIndex = Some (PE entry) ->  *)
+StateLib.getNbLevel = Some level ->
+(* negb presentvaChild = true ->  *)
+In phyDescChild (getPartitions multiplexer s) ->
+(*  isPE ptVaChildpd (StateLib.getIndexOfAddr vaChild fstLevel) s ->
+ getTableAddrRoot ptVaChildpd PDidx phyDescChild vaChild s ->  *)
+ (defaultPage =? ptVaChildpd) = false ->
+ StateLib.getIndexOfAddr vaChild fstLevel = idxvaChild ->
+(*  entryPresentFlag ptVaChildpd idxvaChild presentvaChild s ->   *)
+nextEntryIsPP phyDescChild PDidx pdChildphy s ->
+pdChildphy <> defaultPage ->
+getIndirection pdChildphy vaChild level (nbLevel - 1) s =
+            Some ptVaChildpd ->
+            nbLevel -1 > 0 ->
+~ In ptVaChildpd (getIndirectionsAux pdChildphy s (nbLevel - 1)).
+Proof.
+intros Hpde Hpresdef Hnodupconf Hconfigdiff (* Hparts *) (* Haccess *) (* Hlookup *) Hlevel
+ (* Hnotpresent *) Hchildpart (* Hpe Htblroot *) Hdefaut Hidx (* Hentrypresent *)
+Hpdchild Hpdchildnotnull Hindchild H0.
+ {  assert(0<nbLevel) by apply nbLevelNotZero.
+      assert(nbLevel - 1 + 1 = nbLevel) by omega.
+ assert(Hprevious : exists prevtab,
+      getIndirection pdChildphy vaChild level (nbLevel - 2) s =
+            Some prevtab /\prevtab <> defaultPage /\  StateLib.readPhyEntry prevtab
+  (StateLib.getIndexOfAddr vaChild (CLevel (level- ((nbLevel - 1) - 1)))) (memory s) =
+Some ptVaChildpd).
+{   revert Hindchild   Hdefaut  (*  H0 *).
+
+
+  assert(Hstooo : level > (nbLevel - 1 -1)).
+  { symmetry in Hlevel. apply getNbLevelEq in Hlevel.
+    subst.
+    unfold CLevel.
+    case_eq(lt_dec (nbLevel - 1) nbLevel );intros.
+    simpl.
+    omega. (*
+    unfold CLevel in H0.
+    rewrite H0 in *.
+    simpl in *.
+     *)
+    omega. }
+
+ 
+  assert(Htpp : 0 < nbLevel -1).
+  { symmetry in Hlevel. apply getNbLevelEq in Hlevel.
+    subst.
+    unfold CLevel.
+    case_eq(lt_dec (nbLevel - 1) nbLevel );intros.
+    simpl.
+    omega.
+    omega.
+   
+     }
+  assert(Hnotdef : pdChildphy <> defaultPage) by intuition.
+  revert Hstooo Htpp Hnotdef.
+  clear.
+ 
+  replace (nbLevel -2) with (nbLevel -1 -1) by omega.  
+  revert pdChildphy level ptVaChildpd.
+  induction (nbLevel-1);simpl.
+  intros.
+  omega.
+  intros.
+  case_eq(StateLib.Level.eqb level fstLevel);intros;
+  rewrite H in *.
+  apply levelEqBEqNatTrue0 in H.
+  omega.
+   case_eq(StateLib.readPhyEntry pdChildphy
+                (StateLib.getIndexOfAddr vaChild level) (memory s));intros;
+    rewrite H0 in *;try now contradict Hindchild.
+    case_eq(defaultPage =? p);intros;rewrite H1 in *.
+    apply beq_nat_false in Hdefaut.
+    inversion Hindchild.
+    subst.
+    now contradict Hdefaut.
+    case_eq(StateLib.Level.pred level );intros;rewrite H2 in *.
+    + replace (n-0) with n by omega.
+    assert(Hooo : n = 0 \/ 0 < n) by omega.
+    destruct Hooo.
+    *
+    subst.
+    simpl in *.
+    exists  pdChildphy;split;trivial.
+    inversion Hindchild.
+    subst.
+    rewrite <- H0.
+    split.  trivial.
+    f_equal.
+    f_equal.
+    rewrite <- minus_n_O.
+    apply CLevelIdentity1.
+    * assert(Hii : l > n - 1  ) .
+    apply levelPredMinus1 in H2.
+    subst.
+   unfold CLevel.
+    case_eq( lt_dec (level - 1) nbLevel );intros.
+    simpl.
+    omega.
+    destruct level.
+    simpl in *.
+    omega.
+    trivial.
+    assert(Hi1 : p <> defaultPage).
+    apply beq_nat_false in H1.
+    intuition.
+    subst.
+    now contradict H1.
+      generalize(IHn p l ptVaChildpd Hii H3 Hi1 Hindchild Hdefaut
+       );clear IHn ; intros iHn .
+       destruct iHn as (prevtab & Hindprev & Hdef & Hread).
+       exists prevtab;split;trivial.
+       intros.
+       assert(Hs :S(n-1) = n) by omega.
+       rewrite <- Hs.
+       simpl.
+       rewrite H.
+       rewrite H0.
+       rewrite H1.
+       rewrite H2;trivial.
+       split;trivial.
+       rewrite <- Hread.
+       f_equal.
+       f_equal.
+       f_equal.
+apply levelPredMinus1 in H2.
+rewrite H2.
+unfold CLevel.
+case_eq(lt_dec (level - 1) nbLevel);intros.
+simpl.
+omega.
+destruct level.
+simpl in *.
+omega.
+trivial.
++ assert(Hnotnone : StateLib.Level.pred level <> None).
+apply levelPredNone;trivial. now contradict Hnotnone.  }
+destruct Hprevious as (prevtab & Hprevtable & Hprevnotnull & Hreadprev).
+apply getIndirectionInGetIndirections2 with prevtab vaChild level;
+simpl; subst;
+trivial.
+omega.
+simpl.
+rewrite <- Hprevtable.
+f_equal.
+omega.
+rewrite H1.
+assert(Hdup :   noDupConfigPagesList s) by intuition.
+apply noDupConfigPagesListNoDupGetIndirections with phyDescChild PDidx;trivial.
+apply Hdup;trivial.
+left;trivial.
+apply beq_nat_false in Hdefaut.
+unfold not;intros;subst.
+now contradict Hdefaut.
+move Hlevel at bottom.
+symmetry in Hlevel.
+
+apply getNbLevelEq in Hlevel.
+rewrite Hlevel.
+unfold CLevel.
+case_eq(lt_dec (nbLevel - 1) nbLevel);intros.
+simpl.
+omega.
+omega.
+}
+Qed.
+Lemma indexDecOrNot :
+forall p1 p2 : index, p1 = p2 \/ p1<>p2.
+Proof.
+destruct p1;simpl in *;subst;destruct p2;simpl in *;subst.
+assert (Heq :i=i0 \/ i<> i0) by omega.
+destruct Heq as [Heq|Heq].
+subst.
+left;f_equal;apply proof_irrelevance.
+right. unfold not;intros.
+inversion H.
+subst.
+now contradict Heq.
+Qed.
+Lemma checkVAddrsEqualityWOOffsetTrueLe  :
+forall stop stopi vaToPrepare vavalue nbL,
+stopi <= stop ->
+StateLib.checkVAddrsEqualityWOOffset stop vaToPrepare vavalue nbL = true ->
+StateLib.checkVAddrsEqualityWOOffset stopi vaToPrepare vavalue nbL = true.
+Proof.
+induction stop;simpl.
+* intros.
+  assert(stopi =0) by omega.
+  subst.
+  simpl;trivial.
+* intros.
+ case_eq(StateLib.Level.eqb nbL fstLevel);intros * Hfst;rewrite Hfst in *.
+  destruct stopi;simpl;trivial.
+  rewrite Hfst;trivial.
+  case_eq(StateLib.Level.pred nbL);intros * Hpred;rewrite Hpred in *.
+  + destruct stopi;simpl;trivial.
+    rewrite Hfst.
+    rewrite Hpred.
+    case_eq(StateLib.getIndexOfAddr vaToPrepare nbL =? StateLib.getIndexOfAddr vavalue nbL);
+      intros * Hva;rewrite Hva in *;try now contradict H0.
+  apply IHstop;trivial.
+  omega.
+ + apply levelPredNone  in Hfst.
+  now contradict Hfst.
+Qed.
+
+ Set Nested Proofs Allowed.
+Lemma indirectionNotInPreviousMMULevelAux vaChild s :
+forall (stop : nat) (pdChildphy : page) (level : level) (ptVaChildpd : page),
+level > stop - 1 ->
+0 < stop ->
+pdChildphy <> defaultPage ->
+getIndirection pdChildphy vaChild level stop s = Some ptVaChildpd ->
+(defaultPage =? ptVaChildpd) = false ->
+exists prevtab : page,
+  getIndirection pdChildphy vaChild level (stop - 1) s = Some prevtab /\
+  prevtab <> defaultPage /\
+  StateLib.readPhyEntry prevtab (StateLib.getIndexOfAddr vaChild (CLevel (level - (stop - 1)))) (memory s) = Some ptVaChildpd.
+  Proof.
+  induction stop;simpl.
+  intros * Hstooo Htpp Hnotdef Hindchild Hdefaut.
+  omega.
+intros * Hstooo Htpp Hnotdef Hindchild Hdefaut.
+  case_eq(StateLib.Level.eqb level fstLevel);intros;
+  rewrite H in *.
+  apply levelEqBEqNatTrue0 in H.
+  omega.
+   case_eq(StateLib.readPhyEntry pdChildphy
+                (StateLib.getIndexOfAddr vaChild level) (memory s));intros;
+    rewrite H0 in *;try now contradict Hindchild.
+    case_eq(defaultPage =? p);intros;rewrite H1 in *.
+    apply beq_nat_false in Hdefaut.
+    inversion Hindchild.
+    subst.
+    now contradict Hdefaut.
+    case_eq(StateLib.Level.pred level );intros;rewrite H2 in *.
+    + replace (stop-0) with stop by omega.
+    assert(Hooo : stop = 0 \/ 0 < stop) by omega.
+    destruct Hooo.
+    *
+    subst.
+    simpl in *.
+    exists  pdChildphy;split;trivial.
+    inversion Hindchild.
+    subst.
+    rewrite <- H0.
+    split.  trivial.
+    f_equal.
+    f_equal.
+    rewrite <- minus_n_O.
+    apply CLevelIdentity1.
+    * assert(Hii : l > stop - 1  ) .
+    apply levelPredMinus1 in H2.
+    subst.
+   unfold CLevel.
+    case_eq( lt_dec (level - 1) nbLevel );intros.
+    simpl.
+    omega.
+    destruct level.
+    simpl in *.
+    omega.
+    trivial.
+    assert(Hi1 : p <> defaultPage).
+    apply beq_nat_false in H1.
+    intuition.
+    subst.
+    now contradict H1.
+      generalize(IHstop p l ptVaChildpd Hii H3 Hi1 Hindchild Hdefaut
+       );clear IHstop ; intros iHn .
+       destruct iHn as (prevtab & Hindprev & Hdef & Hread).
+       exists prevtab;split;trivial.
+       intros.
+       assert(Hs :S(stop-1) = stop) by omega.
+       rewrite <- Hs.
+       simpl.
+       rewrite H.
+       rewrite H0.
+       rewrite H1.
+       rewrite H2;trivial.
+       split;trivial.
+       rewrite <- Hread.
+       f_equal.
+       f_equal.
+       f_equal.
+apply levelPredMinus1 in H2.
+rewrite H2.
+unfold CLevel.
+case_eq(lt_dec (level - 1) nbLevel);intros.
+simpl.
+omega.
+destruct level.
+simpl in *.
+omega.
+trivial.
++ assert(Hnotnone : StateLib.Level.pred level <> None).
+apply levelPredNone;trivial. now contradict Hnotnone.
+Qed.
+Lemma indirectionNotInPreviousMMULevel s ptVaChildpd idxvaChild phyVaChild  
+  pdChildphy currentPart
+presentvaChild vaChild phyDescChild level entry:
+ partitionDescriptorEntry s ->
+ isPresentNotDefaultIff s ->
+ noDupConfigPagesList s ->
+configTablesAreDifferent s ->
+In currentPart (getPartitions multiplexer s) ->
+In phyVaChild (getAccessibleMappedPages currentPart s) ->
+lookup ptVaChildpd idxvaChild (memory s) beqPage beqIndex = Some (PE entry) ->
+StateLib.getNbLevel = Some level ->
+negb presentvaChild = true ->
+In phyDescChild (getPartitions multiplexer s) ->
+ isPE ptVaChildpd (StateLib.getIndexOfAddr vaChild fstLevel) s ->
+ getTableAddrRoot ptVaChildpd PDidx phyDescChild vaChild s ->
+ (defaultPage =? ptVaChildpd) = false ->
+ StateLib.getIndexOfAddr vaChild fstLevel = idxvaChild ->
+ entryPresentFlag ptVaChildpd idxvaChild presentvaChild s ->  
+nextEntryIsPP phyDescChild PDidx pdChildphy s ->
+pdChildphy <> defaultPage ->
+getIndirection pdChildphy vaChild level (nbLevel - 1) s =
+            Some ptVaChildpd ->
+            nbLevel -1 > 0 ->
+~ In ptVaChildpd (getIndirectionsAux pdChildphy s (nbLevel - 1)).
+Proof.
+intros Hpde Hpresdef Hnodupconf Hconfigdiff Hparts Haccess Hlookup Hlevel
+ Hnotpresent Hchildpart Hpe Htblroot Hdefaut Hidx Hentrypresent
+Hpdchild Hpdchildnotnull Hindchild H0.
+ assert(0<nbLevel) by apply nbLevelNotZero.
+      assert(nbLevel - 1 + 1 = nbLevel) by omega.
+ assert(Hprevious : exists prevtab,
+      getIndirection pdChildphy vaChild level (nbLevel - 2) s =
+            Some prevtab /\prevtab <> defaultPage /\  StateLib.readPhyEntry prevtab
+  (StateLib.getIndexOfAddr vaChild (CLevel (level- ((nbLevel - 1) - 1)))) (memory s) =
+Some ptVaChildpd).
+{   revert Hindchild   Hdefaut  (*  H0 *).
+
+
+  assert(Hstooo : level > (nbLevel - 1 -1)).
+  { symmetry in Hlevel. apply getNbLevelEq in Hlevel.
+    subst.
+    unfold CLevel.
+    case_eq(lt_dec (nbLevel - 1) nbLevel );intros.
+    simpl.
+    omega. (*
+    unfold CLevel in H0.
+    rewrite H0 in *.
+    simpl in *.
+     *)
+    omega. }
+
+ 
+  assert(Htpp : 0 < nbLevel -1).
+  { symmetry in Hlevel. apply getNbLevelEq in Hlevel.
+    subst.
+    unfold CLevel.
+    case_eq(lt_dec (nbLevel - 1) nbLevel );intros.
+    simpl.
+    omega.
+    omega.
+   
+     }
+  assert(Hnotdef : pdChildphy <> defaultPage) by intuition.
+  revert Hstooo Htpp Hnotdef.
+  clear.
+ 
+  replace (nbLevel -2) with (nbLevel -1 -1) by omega.
+  revert pdChildphy level ptVaChildpd.
+ 
+  generalize   (nbLevel - 1 ) as stop.
+  apply indirectionNotInPreviousMMULevelAux.
+   }
+destruct Hprevious as (prevtab & Hprevtable & Hprevnotnull & Hreadprev).
+apply getIndirectionInGetIndirections2 with prevtab vaChild level;
+simpl; subst;
+trivial.
+omega.
+simpl.
+rewrite <- Hprevtable.
+f_equal.
+omega.
+rewrite H1.
+assert(Hdup :   noDupConfigPagesList s) by intuition.
+apply noDupConfigPagesListNoDupGetIndirections with phyDescChild PDidx;trivial.
+apply Hdup;trivial.
+left;trivial.
+apply beq_nat_false in Hdefaut.
+unfold not;intros;subst.
+now contradict Hdefaut.
+move Hlevel at bottom.
+symmetry in Hlevel.
+
+apply getNbLevelEq in Hlevel.
+rewrite Hlevel.
+unfold CLevel.
+case_eq(lt_dec (nbLevel - 1) nbLevel);intros.
+simpl.
+omega.
+omega.
+Qed.
+
+Lemma pageTablesAreDifferentMiddle stop0 s:
+
+True ->
+forall (n : nat) (root1 root2 table1 table2 : page) (level1 : level) (va1 va2 : vaddr) (stop : nat),
+NoDup (getIndirectionsAux root1 s n) ->
+NoDup (getIndirectionsAux root2 s n) ->
+StateLib.checkVAddrsEqualityWOOffset (S stop0) va1 va2 level1 = false ->
+level1 = CLevel (n - 1) /\ root1 = root2 \/
+level1 < CLevel (n - 1) /\
+(disjoint (getIndirectionsAux root1 s n) (getIndirectionsAux root2 s n) /\ root1 <> root2 \/ root1 = root2) ->
+table1 <> defaultPage ->
+table2 <> defaultPage ->
+getIndirection root1 va1 level1 (S stop0) s = Some table1 ->
+getIndirection root2 va2 level1 (S stop0) s = Some table2 ->
+S stop0 <= stop ->
+root1 <> defaultPage -> root2 <> defaultPage -> S stop0 <= level1 -> n <= nbLevel -> table1 <> table2.
+Proof. intro H0.   induction (S stop0);
+  intros  * HNoDup1 HNoDup2 Hvas Hlevel Hnotnull1 Hnotnull2
+  Htableroot1 (* Hstop *) Htableroot2 (* H0 *) Hs Hroot1 Hroot2 (* Hroot12 *) Hzero Hnbl.
+  simpl in *. now contradict Hvas.
+  intros.
+  simpl in *.
+  case_eq (StateLib.Level.eqb level1 fstLevel); intros ;rewrite H in *.
+  -  apply levelEqBEqNatTrue0 in H.
+  omega.
+  -
+    clear H.
+    case_eq (StateLib.readPhyEntry root1 (StateLib.getIndexOfAddr va1 level1) (memory s)) ;
+    [intros p Hread1 | intros Hread1];
+    rewrite Hread1 in *; [ | inversion Htableroot1].  
+    case_eq (StateLib.readPhyEntry root2 (StateLib.getIndexOfAddr va2 level1) (memory s) );
+    [intros p0 Hread2 | intros Hread2];
+    rewrite Hread2 in *; [ | inversion Htableroot2].
+    case_eq (defaultPage =? p); intros Hnull1;
+    rewrite Hnull1 in *.
+    inversion Htableroot1.
+    subst. now contradict Hnotnull1.
+    case_eq (defaultPage =? p0); intros Hnull2;
+    rewrite Hnull2 in *.
+    inversion Htableroot2.
+    subst. now contradict Hnotnull2.
+    case_eq(StateLib.Level.pred level1); [intros pred Hpred | intros Hpred];  rewrite Hpred in *;
+    [ | inversion Htableroot1].    
+    case_eq (StateLib.getIndexOfAddr va1 level1 =? StateLib.getIndexOfAddr va2 level1);
+            intros Hidx;
+            rewrite Hidx in Hvas; trivial.
+    * generalize (IHn (n0 -1) p p0 table1 table2 pred va1 va2 stop); clear IHn; intros IHn.
+      assert (StateLib.Level.eqb level1 fstLevel = true \/ StateLib.Level.eqb level1 fstLevel = false).
+      { unfold StateLib.Level.eqb.
+        rewrite NPeano.Nat.eqb_eq.  rewrite NPeano.Nat.eqb_neq.
+        omega. }
+      destruct H.
+      { apply levelEqBEqNatTrue in H. subst.
+        unfold StateLib.Level.pred in Hpred.
+        unfold fstLevel in Hpred.
+        unfold CLevel in Hpred.
+        case_eq (lt_dec 0 nbLevel ); intros;
+        rewrite H in Hpred; [simpl in *;inversion Hpred |
+        assert (0 < nbLevel) by apply nbLevelNotZero;
+        now contradict H1]. }
+      { apply IHn;trivial; try omega; clear IHn.
+        + apply nodupLevelMinus1  with root1 (StateLib.getIndexOfAddr va1 level1); trivial.
+          apply beq_nat_false in Hnull1.
+          unfold not. intros.
+          contradict Hnull1. subst. trivial.
+        + apply nodupLevelMinus1  with root2 (StateLib.getIndexOfAddr va2 level1); trivial.
+          apply beq_nat_false in Hnull2.
+          unfold not. intros.
+          contradict Hnull2. subst. trivial.
+        + destruct Hlevel as [(Hlevel& Hroot) | Hlevel ].
+          - left.
+            split.
+            apply levelPredMinus1 in Hpred; trivial.
+            unfold CLevel in Hpred.
+            case_eq(lt_dec (level1 - 1) nbLevel ); intros;
+            rewrite H1 in Hpred.
+            destruct level1. simpl in *.
+            destruct pred.
+            inversion Hpred. subst.
+            apply levelEqBEqNatFalse0 in H.
+            simpl in *.
+            clear Htableroot2 Htableroot1 Hvas Hidx
+            Hread2  Hread1 HNoDup2 HNoDup1
+            Hnull1 Hnull2 Hnotnull2 Hnotnull1 Hroot2 Hroot1.
+            unfold CLevel in *.
+            case_eq (lt_dec (n0 - 1) nbLevel);
+            intros; rewrite H2 in *.
+            simpl in *.
+            case_eq (lt_dec (n0 - 1 - 1) nbLevel);
+            intros.
+            inversion Hlevel. subst.
+            assert(Hl0 = ADT.CLevel_obligation_1 (n0 - 1 - 1) l2 ) by apply proof_irrelevance.
+            subst. reflexivity.
+            simpl in *. omega. omega.
+            destruct level1.
+            simpl in *.
+            omega.
+            subst.
+            apply beq_nat_true in Hidx.
+            destruct (StateLib.getIndexOfAddr va2 (CLevel (n0 - 1))).
+            destruct (StateLib.getIndexOfAddr va1 (CLevel (n0 - 1))).
+            simpl in *.
+            subst. assert (Hi = Hi0) by apply proof_irrelevance.
+            subst. rewrite Hread1 in Hread2.
+            inversion Hread2. trivial.
+          - destruct Hlevel as (Hlevellt &  [(Hlevel & Hll) | Hlevel ]).
+            * right. split.
+              { apply levelPredMinus1 in Hpred; trivial.
+                unfold CLevel in Hpred.
+                case_eq(lt_dec (level1 - 1) nbLevel ); intros;
+                rewrite H1 in Hpred.
+                destruct level1. simpl in *.
+                inversion Hpred. subst.
+                apply levelEqBEqNatFalse0 in H.
+                simpl in *.
+                clear H2 Htableroot2 Htableroot1 Hvas Hidx
+                Hread2  Hread1 Hlevel HNoDup2 HNoDup1 H0
+                Hnull1 Hnull2 Hnotnull2 Hnotnull1 Hroot2 Hroot1.
+                unfold CLevel in *.
+                case_eq (lt_dec (n0 - 1) nbLevel);
+                intros; rewrite H0 in *.
+                simpl in *.
+                case_eq (lt_dec (n0 - 1 - 1) nbLevel);
+                intros.
+                simpl in *.
+                 
+                  omega. omega.  
+                case_eq (lt_dec (n0 - 1 - 1) nbLevel);
+                intros.
+                simpl in *. omega. omega.
+                destruct level1. simpl in *. omega. }
+              { assert (n0 <= 1 \/ n0 > 1) as Hn0. omega.
+                destruct Hn0.
+                apply levelEqBEqNatFalse0 in H.
+                assert (CLevel
+                (n0 - 1) > 1).
+                omega.
+                contradict H1.
+                unfold CLevel in Hlevellt, H2.
+                case_eq ( lt_dec (n0 - 1) nbLevel); intros;  rewrite H1 in *;
+                simpl in *. omega.
+                apply le_lt_or_eq in Hnbl.
+                destruct Hnbl.
+                omega.
+                assert (n0 > 0).
+                assert (0 < nbLevel) by apply nbLevelNotZero.
+                omega.
+                omega.
+                left. split.
+                apply inclDisjoint with (getIndirectionsAux root1 s n0) (getIndirectionsAux root2 s n0); trivial.
+                apply inclGetIndirectionsAuxMinus1 with (StateLib.getIndexOfAddr va1 level1); trivial.
+                apply inclGetIndirectionsAuxMinus1 with (StateLib.getIndexOfAddr va2 level1); trivial.
+                assert (In p (getIndirectionsAux root1 s n0) ) as Hp.
+                apply readPhyEntryInGetIndirectionsAux; trivial.
+                apply beq_nat_false in Hnull1. unfold not. contradict Hnull1.
+                subst. trivial.
+                apply readPhyEntryInGetTablePages with (StateLib.getIndexOfAddr va1 level1); trivial.
+                destruct (StateLib.getIndexOfAddr va1 level1 ); simpl in *; trivial.
+                apply beq_nat_false in Hnull1. unfold not. contradict Hnull1.
+                subst. trivial.
+                assert ((StateLib.getIndexOfAddr va1 level1) = (CIndex (StateLib.getIndexOfAddr va1 level1))).
+                symmetry. apply indexEqId. rewrite <- H2. assumption.
+                generalize(Hlevel p  Hp); intros Hpage0.
+                assert (In p0 (getIndirectionsAux root2 s n0) ) as Hp0.
+                apply readPhyEntryInGetIndirectionsAux; trivial.
+                apply beq_nat_false in Hnull2. unfold not. contradict Hnull2.
+                subst. trivial.
+                apply readPhyEntryInGetTablePages with (StateLib.getIndexOfAddr va2 level1); trivial.
+                destruct (StateLib.getIndexOfAddr va2 level1 ); simpl in *; trivial.
+                apply beq_nat_false in Hnull2. unfold not. contradict Hnull2.
+                subst. trivial.
+                assert ((StateLib.getIndexOfAddr va2 level1) = (CIndex (StateLib.getIndexOfAddr va2 level1))) as Hcidx.
+                symmetry. apply indexEqId. rewrite <- Hcidx. assumption.
+                destruct (getIndirectionsAux root2 s n0). simpl in *. now contradict Hp0.
+                simpl in *. unfold not in *.
+                intros. apply Hpage0.
+                destruct Hp0. subst. left. trivial.
+                subst.
+                right; trivial. }
+            * right. split.
+              apply levelPredMinus1 in Hpred; trivial.
+              unfold CLevel in Hpred.
+              case_eq(lt_dec (level1 - 1) nbLevel ); intros;
+              rewrite H1 in Hpred.
+              destruct level1. simpl in *.
+              inversion Hpred. subst.
+              apply levelEqBEqNatFalse0 in H.
+              simpl in *.
+              clear H2 Htableroot2 Htableroot1 Hvas Hidx
+              Hread2  Hread1 HNoDup2 HNoDup1 H0
+              Hnull1 Hnull2 Hnotnull2 Hnotnull1 Hroot2 Hroot1.
+              unfold CLevel in *.
+              case_eq (lt_dec (n0 - 1) nbLevel);
+              intros; rewrite H0 in *.
+              simpl in *.
+              case_eq (lt_dec (n0 - 1 - 1) nbLevel);
+              intros.
+              simpl in *. omega. omega.  
+              case_eq (lt_dec (n0 - 1 - 1) nbLevel);
+              intros;
+              simpl in *. contradict H0. omega. omega.
+              destruct level1. simpl in *. omega.
+              right.
+              subst.
+              apply beq_nat_true in Hidx.
+              destruct (StateLib.getIndexOfAddr va2 level1).
+              destruct (StateLib.getIndexOfAddr va1 level1).
+              simpl in *.
+              subst. assert (Hi = Hi0) by apply proof_irrelevance.
+              subst. rewrite Hread1 in Hread2.
+              inversion Hread2. trivial.  
+        + apply beq_nat_false in Hnull1.
+          unfold not. intros.
+          contradict Hnull1. subst. trivial.
+        + apply beq_nat_false in Hnull2.
+          unfold not. intros.
+          contradict Hnull2. subst. trivial.
+        + apply levelPredMinus1 in Hpred; trivial.
+          unfold CLevel in Hpred.
+          case_eq(lt_dec (level1 - 1) nbLevel ); intros;
+          rewrite H1 in Hpred.
+          destruct level1. simpl in *.
+          inversion Hpred. subst.
+          apply levelEqBEqNatFalse0 in H.
+          simpl in *.
+          omega.
+          destruct level1;simpl in *.
+          omega.
+         }
+    * clear IHn.
+      clear stop0 stop (* Hstop *) Hs Hvas .
+      destruct Hlevel as [(Hlevel& Hroot) | (Hlevel& [(Hroot & Heq) | Hroot] ) ]; subst.
+      { assert (n0 <= 1 \/ n0 > 1) as Hn0. omega.
+        destruct Hn0 as [Hn0 | Hn0].
+        + assert(n0 = 0 \/ n0 =1) as Hn01. omega.
+          destruct Hn01;subst;  simpl in *;
+          unfold StateLib.Level.pred in *; [
+          case_eq(gt_dec (CLevel 0) 0 ); intros g Hnb0;rewrite Hnb0 in Hpred;
+          [ | now contradict Hpred];
+          unfold CLevel in g |].
+          case_eq (lt_dec 0 nbLevel); intros nbl0 Hnbl0;
+          [ |
+          assert(0 < nbLevel) by apply nbLevelNotZero; omega].
+          clear Hpred Hnb0.
+          rewrite Hnbl0 in *; simpl in *.  now contradict g.
+          case_eq(gt_dec (CLevel 0) 0 ); intros g Hnb0;rewrite Hnb0 in Hpred;
+          [ |
+          now contradict Hpred].
+          unfold CLevel in g.
+          case_eq (lt_dec 0 nbLevel); intros nbl0 Hnbl0; [ |
+          assert(0 < nbLevel) by apply nbLevelNotZero; omega].
+          clear Hpred Hnb0.
+          rewrite Hnbl0 in *; simpl in *.  now contradict g.
+       + assert( p0 <> p).
+          { apply getTablePagesNoDup with root2 (StateLib.getIndexOfAddr va2 (CLevel (n0 - 1)))
+          (StateLib.getIndexOfAddr va1 (CLevel (n0 - 1))) s; trivial.  
+          destruct (StateLib.getIndexOfAddr va2 (CLevel (n0 - 1))). simpl in *; trivial.
+          destruct (StateLib.getIndexOfAddr va1 (CLevel (n0 - 1))). simpl in *; trivial.
+          destruct n0; [now contradict Hn0 |].
+          simpl in HNoDup2. apply NoDup_cons_iff in HNoDup2.
+          destruct HNoDup2 as (_ & HNoDup2).
+          apply getTablePagesNoDupFlatMap  with n0; trivial. omega.
+          assert (H :(CIndex (StateLib.getIndexOfAddr va2 (CLevel (n0 - 1)))) =
+          (StateLib.getIndexOfAddr va2 (CLevel (n0 - 1)))).
+          apply indexEqId. rewrite H; trivial.
+          assert (H2 :(CIndex (StateLib.getIndexOfAddr va1 (CLevel (n0 - 1)))) =
+          (StateLib.getIndexOfAddr va1 (CLevel (n0 - 1)))).
+          apply indexEqId. rewrite H2. trivial.
+          apply NPeano.Nat.eqb_neq. unfold not. intros. rewrite H in Hidx.
+          apply beq_nat_false in Hidx. now contradict Hidx.
+          apply beq_nat_false in Hnull1.
+          apply NPeano.Nat.eqb_neq. unfold not. intros. rewrite H in *.
+          now contradict Hnull1.
+          apply NPeano.Nat.eqb_neq. unfold not. intros. rewrite H in *.
+          apply beq_nat_false in Hnull2. now contradict Hnull2. }
+        assert( disjoint (getIndirectionsAux p s (n0 -1))
+       (getIndirectionsAux p0 s (n0 -1))) as Hdisjoint.
+         apply disjointGetIndirectionsAuxMiddle with root2
+         (StateLib.getIndexOfAddr va2 (CLevel (n0 - 1)))
+         (StateLib.getIndexOfAddr va1 (CLevel (n0 - 1))) ; trivial.
+         assert (In table1 (getIndirectionsAux  p s (n0 -1))) as Htbl1p.
+         apply getIndirectionInGetIndirectionAuxMinus1 with va1 pred n (CLevel (n0 - 1)); trivial.
+         unfold CLevel.
+         case_eq( lt_dec (n0 - 1) nbLevel). intros. simpl.
+         omega.
+         intros.
+         contradict H1. omega.
+         assert (In table2 (getIndirectionsAux  p0 s (n0 -1))) as Htb2p0.
+         apply getIndirectionInGetIndirectionAuxMinus1 with va2 pred n (CLevel (n0 - 1)); trivial.
+         unfold CLevel.
+         case_eq( lt_dec (n0 - 1) nbLevel). intros. simpl.
+         omega.
+         intros.
+         contradict H1. omega.
+         unfold disjoint in *.
+         apply Hdisjoint in Htbl1p.
+         unfold not. intros.
+         apply Htbl1p. subst.
+         assumption. }
+      { assert (n0 <= 1 \/ n0 > 1) as Hn0. omega.
+        destruct Hn0 as [Hn0 | Hn0].
+        + assert(n0 = 0 \/ n0 =1) as Hn01. omega.
+          destruct Hn01;subst;  simpl in *;
+          destruct level1; simpl in *;
+          unfold CLevel in Hlevel;
+          case_eq ( lt_dec 0 nbLevel); intros; rewrite H in *;
+          simpl in *; omega.
+        +  assert (level1 > 0).
+             {unfold StateLib.Level.pred in *.
+         case_eq (  gt_dec level1 0) ; intros;
+         rewrite H in *.
+         inversion Hpred.
+         destruct pred.
+         destruct level1. simpl in *.
+         inversion H2. omega.
+         inversion Hpred.
+         }
+        assert (In table1 (getIndirectionsAux  p s (n0 -1))) as Htbl1p.
+         apply getIndirectionInGetIndirectionAuxMinus1 with va1 pred n level1; trivial.
+         omega.
+          assert (In table2 (getIndirectionsAux  p0 s (n0 -1))) as Htbl2p0.
+         apply getIndirectionInGetIndirectionAuxMinus1 with va2 pred n level1; trivial.
+          omega.
+
+          apply inclGetIndirectionsAuxMinus1 with n0 root1 (StateLib.getIndexOfAddr va1 level1)
+           p s in Hread1; trivial.
+           apply inclGetIndirectionsAuxMinus1 with n0 root2 (StateLib.getIndexOfAddr va2 level1)
+           p0 s in Hread2; trivial.
+           unfold incl, disjoint in *.
+           apply Hread1 in Htbl1p.
+           apply Hread2 in Htbl2p0.
+           apply Hroot in Htbl1p.
+           unfold not. intros.
+           apply Htbl1p. subst.
+           assumption.  
+            }
+        { assert (n0 <= 1 \/ n0 > 1) as Hn0. omega.
+        destruct Hn0 as [Hn0 | Hn0].
+        + assert(n0 = 0 \/ n0 =1) as Hn01. omega.
+        destruct Hn01;subst;  simpl in *;
+          destruct level1; simpl in *;
+          unfold CLevel in Hlevel;
+          case_eq ( lt_dec 0 nbLevel); intros; rewrite H in *;
+          simpl in *; omega.
+         
+       + assert( p0 <> p).
+         { apply getTablePagesNoDup with root2 (StateLib.getIndexOfAddr va2 level1)
+          (StateLib.getIndexOfAddr va1 level1) s; trivial.  
+          destruct (StateLib.getIndexOfAddr va2 level1). simpl in *; trivial.
+          destruct (StateLib.getIndexOfAddr va1 level1). simpl in *; trivial.
+          destruct n0; [now contradict Hn0 |].
+          simpl in HNoDup2. apply NoDup_cons_iff in HNoDup2.
+          destruct HNoDup2 as (_ & HNoDup2).
+          apply getTablePagesNoDupFlatMap  with n0; trivial. omega.
+          assert (H :(CIndex (StateLib.getIndexOfAddr va2 level1)) =
+          (StateLib.getIndexOfAddr va2 level1)).
+          apply indexEqId. rewrite H; trivial.
+          assert (H2 :(CIndex (StateLib.getIndexOfAddr va1 level1)) =
+          (StateLib.getIndexOfAddr va1 level1)).
+          apply indexEqId. rewrite H2. trivial.
+          apply NPeano.Nat.eqb_neq. unfold not. intros. rewrite H in Hidx.
+          apply beq_nat_false in Hidx. now contradict Hidx.
+          apply beq_nat_false in Hnull1.
+          apply NPeano.Nat.eqb_neq. unfold not. intros. rewrite H in *.
+          now contradict Hnull1.
+          apply NPeano.Nat.eqb_neq. unfold not. intros. rewrite H in *.
+          apply beq_nat_false in Hnull2. now contradict Hnull2. }
+      assert( disjoint (getIndirectionsAux p s (n0 -1))
+       (getIndirectionsAux p0 s (n0 -1))) as Hdisjoint.
+         apply disjointGetIndirectionsAuxMiddle with root2
+         (StateLib.getIndexOfAddr va2 level1)
+         (StateLib.getIndexOfAddr va1 level1) ; trivial.
+         assert (In table1 (getIndirectionsAux  p s (n0 -1))) as Htbl1p.
+         apply getIndirectionInGetIndirectionAuxMinus1 with va1 pred n level1; trivial.
+         unfold StateLib.Level.pred in *.
+         case_eq (  gt_dec level1 0) ; intros;
+         rewrite H1 in *.
+         inversion Hpred.
+         destruct pred.
+         destruct level1. simpl in *.
+         inversion H3. omega.
+         inversion Hpred.
+         omega.
+         assert (In table2 (getIndirectionsAux  p0 s (n0 -1))) as Htb2p0.
+         apply getIndirectionInGetIndirectionAuxMinus1 with va2 pred n level1; trivial.
+         unfold StateLib.Level.pred in *.
+         case_eq (  gt_dec level1 0) ; intros;
+         rewrite H1 in *.
+         inversion Hpred.
+         destruct pred.
+         destruct level1. simpl in *.
+         inversion H3. omega.
+         inversion Hpred.
+         omega.
+         unfold disjoint in *.
+         apply Hdisjoint in Htbl1p.
+         unfold not. intros.
+         apply Htbl1p. subst.
+         assumption. }
+Qed.
+Lemma pageTablesOrIndicesAreDifferentMiddle stop0 s:
+
+True ->
+forall (n : nat) (root1 root2 table1 table2 : page) (level1 : level) (va1 va2 : vaddr) (* (stop : nat) *) ,
+NoDup (getIndirectionsAux root1 s n) ->
+NoDup (getIndirectionsAux root2 s n) ->
+StateLib.checkVAddrsEqualityWOOffset (S stop0) va1 va2 level1 = false ->
+level1 = CLevel (n - 1) /\ root1 = root2 \/
+level1 < CLevel (n - 1) /\
+(disjoint (getIndirectionsAux root1 s n) (getIndirectionsAux root2 s n) /\ root1 <> root2 \/ root1 = root2) ->
+table1 <> defaultPage ->
+table2 <> defaultPage ->
+getIndirection root1 va1 level1 stop0 s = Some table1 ->
+getIndirection root2 va2 level1 stop0 s = Some table2 ->
+(* S stop0 <= stop -> *)
+root1 <> defaultPage -> root2 <> defaultPage -> S stop0 <= level1 -> n <= nbLevel ->
+table1 <> table2 \/
+StateLib.getIndexOfAddr va1 (CLevel (level1 -stop0)) <> StateLib.getIndexOfAddr va2 (CLevel (level1 -stop0)) .
+Proof. intro H0.
+intros * HNoDup1 HNoDup2 Hvas Hlevel Hnotnull1 Hnotnull2
+  Htableroot1 (* Hstop *) Htableroot2 (* H0 *)  (* Hs *) Hroot1 Hroot2 (* Hroot12 *) Hzero Hnbl.  
+
+assert(Hs: exists stop , S stop0 <= stop).
+exists (S (S stop0)).
+omega.
+destruct Hs as (stop & Hs).
+revert  HNoDup1 HNoDup2 Hvas Hlevel Hnotnull1 Hnotnull2
+  Htableroot1 (* Hstop *) Htableroot2 (* H0 *)   Hs Hroot1 Hroot2 (* Hroot12 *) Hzero Hnbl.
+revert n  root1 root2 table1 table2 level1 va1 va2 stop.
+ induction stop0;
+  intros *  HNoDup1 HNoDup2 Hvas Hlevel Hnotnull1 Hnotnull2
+  Htableroot1 (* Hstop *) Htableroot2 (* H0 *)  Hs  Hroot1 Hroot2 (* Hroot12 *) Hzero Hnbl.
+  simpl in *.
+  +
+  case_eq( StateLib.getIndexOfAddr va1 level1 =? StateLib.getIndexOfAddr va2 level1);intros Hv;
+  rewrite Hv in *.
+  *   case_eq (StateLib.Level.eqb level1 fstLevel); intros; rewrite H in *;try now contradict Hvas.
+  case_eq(StateLib.Level.pred level1);intros * Hlv;rewrite Hlv in *;try now contradict Hvas.
+  * right. apply beq_nat_false in Hv.
+   replace (CLevel (level1 - 0)) with level1. unfold not;intros Hx;rewrite Hx in *.
+   now contradict Hv.
+   rewrite Nat.sub_0_r.
+   symmetry. apply
+    CLevelIdentity1.
+  + simpl in *.
+  case_eq (StateLib.Level.eqb level1 fstLevel); intros ;rewrite H in *.
+  -  apply levelEqBEqNatTrue0 in H.
+  omega.
+  -
+    clear H.
+    case_eq (StateLib.readPhyEntry root1 (StateLib.getIndexOfAddr va1 level1) (memory s)) ;
+    [intros p Hread1 | intros Hread1];
+    rewrite Hread1 in *; [ | inversion Htableroot1].  
+    case_eq (StateLib.readPhyEntry root2 (StateLib.getIndexOfAddr va2 level1) (memory s) );
+    [intros p0 Hread2 | intros Hread2];
+    rewrite Hread2 in *; [ | inversion Htableroot2].
+    case_eq (defaultPage =? p); intros Hnull1;
+    rewrite Hnull1 in *.
+    inversion Htableroot1.
+    subst. now contradict Hnotnull1.
+    case_eq (defaultPage =? p0); intros Hnull2;
+    rewrite Hnull2 in *.
+    inversion Htableroot2.
+    subst. now contradict Hnotnull2.
+    case_eq(StateLib.Level.pred level1); [intros pred Hpred | intros Hpred];  rewrite Hpred in *;
+    [ | inversion Htableroot1].    
+    case_eq (StateLib.getIndexOfAddr va1 level1 =? StateLib.getIndexOfAddr va2 level1);
+            intros Hidx;
+            rewrite Hidx in Hvas; trivial.
+    * generalize (IHstop0  (n-1) p p0 table1 table2 pred va1 va2  stop); clear IHstop0; intros IHn.
+      assert (StateLib.Level.eqb level1 fstLevel = true \/ StateLib.Level.eqb level1 fstLevel = false).
+      { unfold StateLib.Level.eqb.
+        rewrite NPeano.Nat.eqb_eq.  rewrite NPeano.Nat.eqb_neq.
+        omega. }
+      destruct H.
+      { apply levelEqBEqNatTrue in H. subst.
+        unfold StateLib.Level.pred in Hpred.
+        unfold fstLevel in Hpred.
+        unfold CLevel in Hpred.
+        case_eq (lt_dec 0 nbLevel ); intros;
+        rewrite H in Hpred; [simpl in *;inversion Hpred |
+        assert (0 < nbLevel) by apply nbLevelNotZero;
+        now contradict H1]. }
+      { replace (CLevel (level1 - S stop0)) with (CLevel (pred - stop0)).
+        2:{  f_equal.
+        apply levelPredMinus1 in Hpred;trivial.
+        rewrite Hpred.
+        apply levelEqBEqNatFalse0 in H.
+        unfold CLevel.
+        case_eq(lt_dec (level1 - 1) nbLevel);intros * Hx;simpl.
+        omega.
+        destruct level1.
+        simpl in *.
+        omega. }
+      apply IHn;trivial; try omega; clear IHn.
+        + apply nodupLevelMinus1  with root1 (StateLib.getIndexOfAddr va1 level1); trivial.
+          apply beq_nat_false in Hnull1.
+          unfold not. intros.
+          contradict Hnull1. subst. trivial.
+        + apply nodupLevelMinus1  with root2 (StateLib.getIndexOfAddr va2 level1); trivial.
+          apply beq_nat_false in Hnull2.
+          unfold not. intros.
+          contradict Hnull2. subst. trivial.
+        + destruct Hlevel as [(Hlevel& Hroot) | Hlevel ].
+          - left.
+            split.
+            apply levelPredMinus1 in Hpred; trivial.
+            unfold CLevel in Hpred.
+            case_eq(lt_dec (level1 - 1) nbLevel ); intros;
+            rewrite H1 in Hpred.
+            destruct level1. simpl in *.
+            destruct pred.
+            inversion Hpred. subst.
+            apply levelEqBEqNatFalse0 in H.
+            simpl in *.
+            clear Htableroot2 Htableroot1 Hvas Hidx
+            Hread2  Hread1 HNoDup2 HNoDup1
+            Hnull1 Hnull2 Hnotnull2 Hnotnull1 Hroot2 Hroot1.
+            unfold CLevel in *.
+            case_eq (lt_dec (n - 1) nbLevel);
+            intros; rewrite H2 in *.
+            simpl in *.
+            case_eq (lt_dec (n - 1 - 1) nbLevel);
+            intros.
+            inversion Hlevel. subst.
+            assert(Hl0 = ADT.CLevel_obligation_1 (n - 1 - 1) l2 ) by apply proof_irrelevance.
+            subst. reflexivity.
+            simpl in *. omega. omega.
+            destruct level1.
+            simpl in *.
+            omega.
+            subst.
+            apply beq_nat_true in Hidx.
+            destruct (StateLib.getIndexOfAddr va2 (CLevel (n - 1))).
+            destruct (StateLib.getIndexOfAddr va1 (CLevel (n - 1))).
+            simpl in *.
+            subst. assert (Hi = Hi0) by apply proof_irrelevance.
+            subst. rewrite Hread1 in Hread2.
+            inversion Hread2. trivial.
+          - destruct Hlevel as (Hlevellt &  [(Hlevel & Hll) | Hlevel ]).
+            * right. split.
+              { apply levelPredMinus1 in Hpred; trivial.
+                unfold CLevel in Hpred.
+                case_eq(lt_dec (level1 - 1) nbLevel ); intros;
+                rewrite H1 in Hpred.
+                destruct level1. simpl in *.
+                inversion Hpred. subst.
+                apply levelEqBEqNatFalse0 in H.
+                simpl in *.
+                clear H2 Htableroot2 Htableroot1 Hvas Hidx
+                Hread2  Hread1 Hlevel HNoDup2 HNoDup1 H0
+                Hnull1 Hnull2 Hnotnull2 Hnotnull1 Hroot2 Hroot1.
+                unfold CLevel in *.
+                case_eq (lt_dec (n - 1) nbLevel);
+                intros; rewrite H0 in *.
+                simpl in *.
+                case_eq (lt_dec (n - 1 - 1) nbLevel);
+                intros.
+                simpl in *.
+                 
+                  omega. omega.  
+                case_eq (lt_dec (n - 1 - 1) nbLevel);
+                intros.
+                simpl in *. omega. omega.
+                destruct level1. simpl in *. omega. }
+              { assert (n <= 1 \/ n > 1) as Hn0. omega.
+                destruct Hn0.
+                apply levelEqBEqNatFalse0 in H.
+                assert (CLevel
+                (n - 1) > 1).
+                omega.
+                contradict H1.
+                unfold CLevel in Hlevellt, H2.
+                case_eq ( lt_dec (n - 1) nbLevel); intros;  rewrite H1 in *;
+                simpl in *. omega.
+                apply le_lt_or_eq in Hnbl.
+                destruct Hnbl.
+                omega.
+                assert (n > 0).
+                assert (0 < nbLevel) by apply nbLevelNotZero.
+                omega.
+                omega.
+                left. split.
+                apply inclDisjoint with (getIndirectionsAux root1 s n) (getIndirectionsAux root2 s n); trivial.
+                apply inclGetIndirectionsAuxMinus1 with (StateLib.getIndexOfAddr va1 level1); trivial.
+                apply inclGetIndirectionsAuxMinus1 with (StateLib.getIndexOfAddr va2 level1); trivial.
+                assert (In p (getIndirectionsAux root1 s n) ) as Hp.
+                apply readPhyEntryInGetIndirectionsAux; trivial.
+                apply beq_nat_false in Hnull1. unfold not. contradict Hnull1.
+                subst. trivial.
+                apply readPhyEntryInGetTablePages with (StateLib.getIndexOfAddr va1 level1); trivial.
+                destruct (StateLib.getIndexOfAddr va1 level1 ); simpl in *; trivial.
+                apply beq_nat_false in Hnull1. unfold not. contradict Hnull1.
+                subst. trivial.
+                assert ((StateLib.getIndexOfAddr va1 level1) = (CIndex (StateLib.getIndexOfAddr va1 level1))).
+                symmetry. apply indexEqId. rewrite <- H2. assumption.
+                generalize(Hlevel p  Hp); intros Hpage0.
+                assert (In p0 (getIndirectionsAux root2 s n) ) as Hp0.
+                apply readPhyEntryInGetIndirectionsAux; trivial.
+                apply beq_nat_false in Hnull2. unfold not. contradict Hnull2.
+                subst. trivial.
+                apply readPhyEntryInGetTablePages with (StateLib.getIndexOfAddr va2 level1); trivial.
+                destruct (StateLib.getIndexOfAddr va2 level1 ); simpl in *; trivial.
+                apply beq_nat_false in Hnull2. unfold not. contradict Hnull2.
+                subst. trivial.
+                assert ((StateLib.getIndexOfAddr va2 level1) = (CIndex (StateLib.getIndexOfAddr va2 level1))) as Hcidx.
+                symmetry. apply indexEqId. rewrite <- Hcidx. assumption.
+                destruct (getIndirectionsAux root2 s n). simpl in *. now contradict Hp0.
+                simpl in *. unfold not in *.
+                intros. apply Hpage0.
+                destruct Hp0. subst. left. trivial.
+                subst.
+                right; trivial. }
+            * right. split.
+              apply levelPredMinus1 in Hpred; trivial.
+              unfold CLevel in Hpred.
+              case_eq(lt_dec (level1 - 1) nbLevel ); intros;
+              rewrite H1 in Hpred.
+              destruct level1. simpl in *.
+              inversion Hpred. subst.
+              apply levelEqBEqNatFalse0 in H.
+              simpl in *.
+              clear H2 Htableroot2 Htableroot1 Hvas Hidx
+              Hread2  Hread1 HNoDup2 HNoDup1 H0
+              Hnull1 Hnull2 Hnotnull2 Hnotnull1 Hroot2 Hroot1.
+              unfold CLevel in *.
+              case_eq (lt_dec (n - 1) nbLevel);
+              intros; rewrite H0 in *.
+              simpl in *.
+              case_eq (lt_dec (n - 1 - 1) nbLevel);
+              intros.
+              simpl in *. omega. omega.  
+              case_eq (lt_dec (n - 1 - 1) nbLevel);
+              intros;
+              simpl in *. contradict H0. omega. omega.
+              destruct level1. simpl in *. omega.
+              right.
+              subst.
+              apply beq_nat_true in Hidx.
+              destruct (StateLib.getIndexOfAddr va2 level1).
+              destruct (StateLib.getIndexOfAddr va1 level1).
+              simpl in *.
+              subst. assert (Hi = Hi0) by apply proof_irrelevance.
+              subst. rewrite Hread1 in Hread2.
+              inversion Hread2. trivial.  
+        + apply beq_nat_false in Hnull1.
+          unfold not. intros.
+          contradict Hnull1. subst. trivial.
+        + apply beq_nat_false in Hnull2.
+          unfold not. intros.
+          contradict Hnull2. subst. trivial.
+        + apply levelPredMinus1 in Hpred; trivial.
+          unfold CLevel in Hpred.
+          case_eq(lt_dec (level1 - 1) nbLevel ); intros;
+          rewrite H1 in Hpred.
+          destruct level1. simpl in *.
+          inversion Hpred. subst.
+          apply levelEqBEqNatFalse0 in H.
+          simpl in *.
+          omega.
+          destruct level1;simpl in *.
+          omega.
+         }
+    * clear IHstop0.
+(*       clear stop0 stop (* Hstop *) Hs Hvas .  *)
+      destruct Hlevel as [(Hlevel& Hroot) | (Hlevel& [(Hroot & Heq) | Hroot] ) ]; subst.
+      { assert (n <= 1 \/ n > 1) as Hn0. omega.
+        destruct Hn0 as [Hn0 | Hn0].
+        + assert(n = 0 \/ n =1) as Hn01. omega.
+          destruct Hn01;subst;  simpl in *;
+          unfold StateLib.Level.pred in *; [
+          case_eq(gt_dec (CLevel 0) 0 ); intros g Hnb0;rewrite Hnb0 in Hpred;
+          [ | now contradict Hpred];
+          unfold CLevel in g |].
+          case_eq (lt_dec 0 nbLevel); intros nbl0 Hnbl0;
+          [ |
+          assert(0 < nbLevel) by apply nbLevelNotZero; omega].
+          clear Hpred Hnb0.
+          rewrite Hnbl0 in *; simpl in *.  now contradict g.
+          case_eq(gt_dec (CLevel 0) 0 ); intros g Hnb0;rewrite Hnb0 in Hpred;
+          [ |
+          now contradict Hpred].
+          unfold CLevel in g.
+          case_eq (lt_dec 0 nbLevel); intros nbl0 Hnbl0; [ |
+          assert(0 < nbLevel) by apply nbLevelNotZero; omega].
+          clear Hpred Hnb0.
+          rewrite Hnbl0 in *; simpl in *.  now contradict g.
+       + assert( p0 <> p).
+          { apply getTablePagesNoDup with root2 (StateLib.getIndexOfAddr va2 (CLevel (n - 1)))
+          (StateLib.getIndexOfAddr va1 (CLevel (n - 1))) s; trivial.  
+          destruct (StateLib.getIndexOfAddr va2 (CLevel (n - 1))). simpl in *; trivial.
+          destruct (StateLib.getIndexOfAddr va1 (CLevel (n - 1))). simpl in *; trivial.
+          destruct n; [now contradict Hn0 |].
+          simpl in HNoDup2. apply NoDup_cons_iff in HNoDup2.
+          destruct HNoDup2 as (_ & HNoDup2).
+          apply getTablePagesNoDupFlatMap  with n; trivial. omega.
+          assert (H :(CIndex (StateLib.getIndexOfAddr va2 (CLevel (n - 1)))) =
+          (StateLib.getIndexOfAddr va2 (CLevel (n - 1)))).
+          apply indexEqId. rewrite H; trivial.
+          assert (H2 :(CIndex (StateLib.getIndexOfAddr va1 (CLevel (n - 1)))) =
+          (StateLib.getIndexOfAddr va1 (CLevel (n - 1)))).
+          apply indexEqId. rewrite H2. trivial.
+          apply NPeano.Nat.eqb_neq. unfold not. intros. rewrite H in Hidx.
+          apply beq_nat_false in Hidx. now contradict Hidx.
+          apply beq_nat_false in Hnull1.
+          apply NPeano.Nat.eqb_neq. unfold not. intros. rewrite H in *.
+          now contradict Hnull1.
+          apply NPeano.Nat.eqb_neq. unfold not. intros. rewrite H in *.
+          apply beq_nat_false in Hnull2. now contradict Hnull2. }
+        assert( disjoint (getIndirectionsAux p s (n -1))
+       (getIndirectionsAux p0 s (n -1))) as Hdisjoint.
+         apply disjointGetIndirectionsAuxMiddle with root2
+         (StateLib.getIndexOfAddr va2 (CLevel (n - 1)))
+         (StateLib.getIndexOfAddr va1 (CLevel (n - 1))) ; trivial.
+         assert (In table1 (getIndirectionsAux  p s (n -1))) as Htbl1p.
+         { apply getIndirectionInGetIndirectionAuxMinus1 with va1 pred stop0 (CLevel (n - 1)); trivial.
+         unfold CLevel.
+         case_eq( lt_dec (n - 1) nbLevel). intros. simpl.
+         omega.
+         intros.
+         contradict H1. omega. }
+         assert (In table2 (getIndirectionsAux  p0 s (n -1))) as Htb2p0.
+         apply getIndirectionInGetIndirectionAuxMinus1 with va2 pred stop0 (CLevel (n - 1)); trivial.
+         unfold CLevel.
+         case_eq( lt_dec (n - 1) nbLevel). intros. simpl.
+         omega.
+         intros.
+         contradict H1. omega.
+         unfold disjoint in *.
+         apply Hdisjoint in Htbl1p.
+         unfold not. intros.
+         left. intros.
+         apply Htbl1p. subst.
+         assumption. }
+      { assert (n <= 1 \/ n > 1) as Hn0. omega.
+        destruct Hn0 as [Hn0 | Hn0].
+        + assert(n = 0 \/ n =1) as Hn01. omega.
+          destruct Hn01;subst;  simpl in *;
+          destruct level1; simpl in *;
+          unfold CLevel in Hlevel;
+          case_eq ( lt_dec 0 nbLevel); intros; rewrite H in *;
+          simpl in *; omega.
+        +  assert (level1 > 0).
+             {unfold StateLib.Level.pred in *.
+         case_eq (  gt_dec level1 0) ; intros;
+         rewrite H in *.
+         inversion Hpred.
+         destruct pred.
+         destruct level1. simpl in *.
+         inversion H2. omega.
+         inversion Hpred.
+         }
+        assert (In table1 (getIndirectionsAux  p s (n -1))) as Htbl1p.
+         apply getIndirectionInGetIndirectionAuxMinus1 with va1 pred stop0 level1; trivial.
+         omega.
+          assert (In table2 (getIndirectionsAux  p0 s (n -1))) as Htbl2p0.
+         apply getIndirectionInGetIndirectionAuxMinus1 with va2 pred stop0 level1; trivial.
+          omega.
+
+          apply inclGetIndirectionsAuxMinus1 with n root1 (StateLib.getIndexOfAddr va1 level1)
+           p s in Hread1; trivial.
+           apply inclGetIndirectionsAuxMinus1 with n root2 (StateLib.getIndexOfAddr va2 level1)
+           p0 s in Hread2; trivial.
+           unfold incl, disjoint in *.
+           apply Hread1 in Htbl1p.
+           apply Hread2 in Htbl2p0.
+           apply Hroot in Htbl1p.
+           unfold not. intros.
+           left;intros.
+           apply Htbl1p. subst.
+           assumption.  
+            }
+        { assert (n <= 1 \/ n > 1) as Hn0. omega.
+        destruct Hn0 as [Hn0 | Hn0].
+        + assert(n = 0 \/ n =1) as Hn01. omega.
+        destruct Hn01;subst;  simpl in *;
+          destruct level1; simpl in *;
+          unfold CLevel in Hlevel;
+          case_eq ( lt_dec 0 nbLevel); intros; rewrite H in *;
+          simpl in *; omega.
+         
+       + assert( p0 <> p).
+         { apply getTablePagesNoDup with root2 (StateLib.getIndexOfAddr va2 level1)
+          (StateLib.getIndexOfAddr va1 level1) s; trivial.  
+          destruct (StateLib.getIndexOfAddr va2 level1). simpl in *; trivial.
+          destruct (StateLib.getIndexOfAddr va1 level1). simpl in *; trivial.
+          destruct n; [now contradict Hn0 |].
+          simpl in HNoDup2. apply NoDup_cons_iff in HNoDup2.
+          destruct HNoDup2 as (_ & HNoDup2).
+          apply getTablePagesNoDupFlatMap  with n; trivial. omega.
+          assert (H :(CIndex (StateLib.getIndexOfAddr va2 level1)) =
+          (StateLib.getIndexOfAddr va2 level1)).
+          apply indexEqId. rewrite H; trivial.
+          assert (H2 :(CIndex (StateLib.getIndexOfAddr va1 level1)) =
+          (StateLib.getIndexOfAddr va1 level1)).
+          apply indexEqId. rewrite H2. trivial.
+          apply NPeano.Nat.eqb_neq. unfold not. intros. rewrite H in Hidx.
+          apply beq_nat_false in Hidx. now contradict Hidx.
+          apply beq_nat_false in Hnull1.
+          apply NPeano.Nat.eqb_neq. unfold not. intros. rewrite H in *.
+          now contradict Hnull1.
+          apply NPeano.Nat.eqb_neq. unfold not. intros. rewrite H in *.
+          apply beq_nat_false in Hnull2. now contradict Hnull2. }
+      assert( disjoint (getIndirectionsAux p s (n -1))
+       (getIndirectionsAux p0 s (n -1))) as Hdisjoint.
+         apply disjointGetIndirectionsAuxMiddle with root2
+         (StateLib.getIndexOfAddr va2 level1)
+         (StateLib.getIndexOfAddr va1 level1) ; trivial.
+         assert (In table1 (getIndirectionsAux  p s (n -1))) as Htbl1p.
+         apply getIndirectionInGetIndirectionAuxMinus1 with va1 pred stop0 level1; trivial.
+         unfold StateLib.Level.pred in *.
+         case_eq (  gt_dec level1 0) ; intros;
+         rewrite H1 in *.
+         inversion Hpred.
+         destruct pred.
+         destruct level1. simpl in *.
+         inversion H3. omega.
+         inversion Hpred.
+         omega.
+         assert (In table2 (getIndirectionsAux  p0 s (n -1))) as Htb2p0.
+         apply getIndirectionInGetIndirectionAuxMinus1 with va2 pred stop0 level1; trivial.
+         unfold StateLib.Level.pred in *.
+         case_eq (  gt_dec level1 0) ; intros;
+         rewrite H1 in *.
+         inversion Hpred.
+         destruct pred.
+         destruct level1. simpl in *.
+         inversion H3. omega.
+         inversion Hpred.
+         omega.
+         unfold disjoint in *.
+         apply Hdisjoint in Htbl1p.
+         unfold not. intros.
+         left;intros.
+         apply Htbl1p. subst.
+         assumption. }
+Qed.
+
+Lemma getIndirectionInGetIndirections2' (stop : nat) s
+(va : vaddr) (level1 : level) (table root : page) :
+(stop+1) <= nbLevel ->
+getIndirection root va level1 stop s = Some table ->
+NoDup (getIndirectionsAux root s (stop+1)) ->
+table <> defaultPage ->
+root <> defaultPage ->
+stop <= level1 ->
+stop > 0 ->
+~ In table (getIndirectionsAux root s stop).
+Proof.
+intros.
+apply indirectionNotInPreviousMMULevelAux in H0;trivial.
+destruct H0 as ( prevtab & Hi1 & Hi2 & Hi3 ).
+apply getIndirectionInGetIndirections2  with prevtab va level1;trivial.
+omega.
+rewrite  Nat.eqb_neq.
+destruct defaultPage;simpl in *;destruct table;simpl in *;intuition.
+subst.
+apply H2.
+f_equal.
+apply proof_irrelevance.
+
+Qed.
+
+
+Lemma checkVAddrsEqualityWOOffsetPermut' n va1 va2 level1 :
+  StateLib.checkVAddrsEqualityWOOffset n va1 va2 level1 =
+  StateLib.checkVAddrsEqualityWOOffset n va2 va1 level1.
+Proof.
+  revert va1 va2 level1.
+  induction n.
+  simpl. trivial.
+  simpl. intros.
+  case_eq (StateLib.Level.eqb level1 fstLevel); intros.
+  apply NPeano.Nat.eqb_sym.
+  case_eq(StateLib.Level.pred level1);
+  intros; trivial.
+  rewrite  NPeano.Nat.eqb_sym.
+  case_eq (StateLib.getIndexOfAddr va2 level1 =? StateLib.getIndexOfAddr va1 level1); intros; trivial.
+Qed.
+
+Lemma getIndirectionInGetIndirections2n:
+  forall stopn (stop : nat) (s : state) (va : vaddr) (level1 : level) (table root : page),
+  stop + 1 <= nbLevel ->
+  getIndirection root va level1 stop s = Some table ->
+  NoDup (getIndirectionsAux root s (stop+1)) ->
+  stopn <= stop ->
+  table <> defaultPage -> root <> defaultPage -> stop <= level1 -> stop > 0 -> ~ In table (getIndirectionsAux root s stopn).
+Proof.
+
+intros.
+apply indirectionNotInPreviousMMULevelAux in H0;trivial.
+destruct H0 as ( prevtab & Hi1 & Hi2 & Hi3 ).
+assert( Hnitin: ~ In table (getIndirectionsAux root s stop)).
+apply getIndirectionInGetIndirections2  with prevtab va level1;trivial.
+contradict Hnitin.
+pose proof inclGetIndirectionsAuxLe as Hii.
+unfold incl in *.
+apply Hii with stopn;trivial.
+omega.
+rewrite  Nat.eqb_neq.
+destruct defaultPage;simpl in *;destruct table;simpl in *;intuition.
+subst.
+apply H3.
+f_equal.
+apply proof_irrelevance.
+Qed.  
+
+Lemma getIndirectionStopLevelGe s va p (l: nat) (level : level)  (l0 : nat) p0:
+ level <=l0 -> l = level ->  
+getIndirection p va level l0 s = Some p0 ->  
+getIndirection p va level l s = Some p0.
+Proof.
+intros.
+revert p0 p level l H H0 H1.
+induction l0;
+intros.
+subst.
+
+
+apply NPeano.Nat.le_0_r in H.
+rewrite H in *;trivial.
+simpl.
+destruct l; simpl in *.
+assert (  StateLib.Level.eqb level fstLevel = true).
+unfold MALInternal.Level.eqb.
+apply NPeano.Nat.eqb_eq.
+rewrite <- H0. unfold fstLevel. unfold CLevel.
+assert ( 0 < nbLevel) by apply nbLevelNotZero.
+case_eq (lt_dec 0 nbLevel ); intros.
+simpl. trivial.
+now contradict H2.
+rewrite H2 in H1. assumption.
+simpl in *.
+case_eq (StateLib.Level.eqb level fstLevel); intros.
+rewrite H2 in H1. destruct l0. simpl. assumption. assumption.  
++ simpl. rewrite H2 in H1.
+  case_eq(StateLib.readPhyEntry p (StateLib.getIndexOfAddr va level) (memory s) ). intros.
+  rewrite H3 in H1.
+  case_eq (defaultPage =? p1); intros;
+  rewrite H4 in H1. assumption.
+  case_eq (StateLib.Level.pred level);
+  intros; rewrite H5 in H1.
+  apply levelPredMinus1 in H5; trivial.
+  unfold CLevel in H5.  
+  case_eq(lt_dec (level - 1) nbLevel ); intros; rewrite H6 in H5.
+  destruct level. simpl in *. subst.
+  simpl in *.
+   
+  apply IHl0 ; trivial. simpl. omega. simpl. omega.
+  destruct level. simpl in *. omega. assumption.
+  intros. rewrite H3 in H1. assumption.
+Qed.
+
+    Lemma CLevelIdentity' : forall l : level, CLevel (l -  0) = l.
+Proof.
+intros l.
+
+simpl.
+rewrite NPeano.Nat.sub_0_r.
+apply CLevelIdentity1.
+Qed.
+
+Lemma checkVAddrsEqualityWOOffsetFalseS:
+forall stop vaToPrepare vavalue , forall (nbL:level),
+StateLib.getIndexOfAddr vaToPrepare (CLevel (nbL - stop)) =
+StateLib.getIndexOfAddr vavalue (CLevel (nbL - stop)) ->
+StateLib.checkVAddrsEqualityWOOffset (stop + 1) vaToPrepare vavalue nbL = false ->
+StateLib.checkVAddrsEqualityWOOffset stop vaToPrepare vavalue nbL = false.
+Proof.
+induction stop;simpl.
+* intros.
+  case_eq(StateLib.Level.eqb nbL fstLevel);intros * Hfst;rewrite Hfst in *.
+  + rewrite CLevelIdentity' in H.
+    rewrite H in H0.
+    rewrite <- beq_nat_refl in H0.
+    trivial.
+  + case_eq(StateLib.Level.pred nbL );intros * Hpred;rewrite Hpred in *;try now contradict H0.
+    rewrite CLevelIdentity' in H.
+    rewrite H in H0.
+    rewrite <- beq_nat_refl in H0.
+    trivial.
+* intros.
+case_eq(StateLib.Level.eqb nbL fstLevel);intros * Hfst;rewrite Hfst in *;trivial.
+case_eq(StateLib.Level.pred nbL );intros * Hpred;rewrite Hpred in *;try now contradict H0;
+trivial.
+case_eq( StateLib.getIndexOfAddr vaToPrepare nbL =? StateLib.getIndexOfAddr vavalue nbL); intros
+* Hvas;rewrite Hvas in *;trivial.
+apply IHstop;trivial.
+ replace (nbL - S stop) with (l - stop) in *.
+ trivial.
+ assert(l = CLevel (nbL - 1)).
+ apply levelPredMinus1;trivial.
+ rewrite H1.
+unfold CLevel .
+case_eq( lt_dec (nbL - 1) nbLevel);intros * Hl;simpl.
+omega.
+destruct nbL. simpl in *. omega.
+Qed.
